add Henkin_constant

theories/Logic/BasicFol2.v
@@ -7,9 +7,9 @@ Require Import PnV.Logic.BasicFol.
 
 #[local] Infix "\in" := E.In.
 #[local] Infix "\subseteq" := E.isSubsetOf.
-#[local] Notation In := List.In.
+#[local] Notation In := L.In.
 
-#[global] Hint Rewrite L.forallb_forall : simplication_hints.
+#[local] Hint Rewrite @L.forallb_forall @Prelude.eqb_spec : simplication_hints.
 
 Import FolNotations.
 
@@ -23,7 +23,7 @@ Definition Henkin_constants : Set := nat.
 
 Context {L : language}.
 
-Let L' : language := augmented_language L Henkin_constants.
+Notation L' := (augmented_language L Henkin_constants).
 
 Fixpoint HC_occurs_in_trm (hc : Henkin_constants) (t : trm L') : bool :=
   match t with
@@ -169,7 +169,7 @@ Qed.
 Lemma last_HC_gt_frm (hc : Henkin_constants)
   : forall p : frm L', hc > maxs (accum_HCs_frm p) -> HC_occurs_in_frm hc p = false.
 Proof.
-  intros p IN. destruct (HC_occurs_in_frm hc p) as [ | ] eqn: H_OBS; trivial.
+  intros p IN. destruct (HC_occurs_in_frm hc p) as [ | ] eqn : H_OBS; trivial.
   rewrite HC_occurs_in_frm_iff_in_accumHCs_frm in H_OBS. enough (WTS : hc <= maxs (accum_HCs_frm p)) by lia.
   eapply in_maxs_ge. exact H_OBS.
 Qed.
@@ -183,6 +183,1048 @@ Proof.
     + eapply last_HC_gt_frm. unfold "∘"%prg in H. lia.
     + eapply IH; trivial. lia.
 Qed.
+
+#[local] Notation hatom := (ivar + Henkin_constants)%type.
+
+#[local] Notation hsubst := (hatom -> trm L').
+
+Section HSUBST.
+
+#[local] Open Scope list_scope.
+
+Definition to_hsubst (s : subst L') : hsubst :=
+  fun z : hatom =>
+  match z with
+  | inl x => s x
+  | inr c => @Con_trm L' (inr c)
+  end.
+
+Definition from_hsubst (sigma : hsubst) : subst L' :=
+  fun z : ivar => sigma (inl z).
+
+Fixpoint accum_hatom_in_trm (t : trm L') : list hatom :=
+  match t with
+  | Var_trm x => [inl x]
+  | Fun_trm f ts => accum_hatom_in_trms ts
+  | Con_trm c =>
+    match c with
+    | inl cc => []
+    | inr hc => [inr hc]
+    end
+  end
+with accum_hatom_in_trms {n : nat} (ts : trms L' n) : list hatom :=
+  match ts with
+  | O_trms => []
+  | S_trms n t ts => accum_hatom_in_trm t ++ accum_hatom_in_trms ts
+  end.
+
+Lemma in_accum_hatom_in_trm_iff_is_free_in_trm x (t : trm L')
+  : L.In (inl x) (accum_hatom_in_trm t) <-> is_free_in_trm x t = true
+with in_accum_hatom_in_trms_iff_is_free_in_trms n x (ts : trms L' n)
+  : L.In (inl x) (accum_hatom_in_trms ts) <-> is_free_in_trms x ts = true.
+Proof.
+  - clear in_accum_hatom_in_trm_iff_is_free_in_trm; revert x. trm_ind t; intros z.
+    + s!. firstorder congruence.
+    + simpl. rewrite is_free_in_trm_unfold. eapply in_accum_hatom_in_trms_iff_is_free_in_trms.
+    + destruct c as [cc | hc]; ss!.
+  - clear in_accum_hatom_in_trms_iff_is_free_in_trms; revert x. trms_ind ts; intros z.
+    + s!. firstorder congruence.
+    + simpl. rewrite is_free_in_trms_unfold. rewrite orb_true_iff. rewrite <- IH with (x := z). rewrite L.in_app_iff. rewrite in_accum_hatom_in_trm_iff_is_free_in_trm. reflexivity.
+Qed.
+
+Lemma in_accum_hatom_in_trm_iff_HC_occurs_in_trm hc (t : trm L')
+  : L.In (inr hc) (accum_hatom_in_trm t) <-> HC_occurs_in_trm hc t = true
+with in_accum_hatom_in_trms_iff_HC_occurs_in_trms n hc (ts : trms L' n)
+  : L.In (inr hc) (accum_hatom_in_trms ts) <-> HC_occurs_in_trms hc ts = true.
+Proof.
+  - clear in_accum_hatom_in_trm_iff_HC_occurs_in_trm; revert hc. trm_ind t; intros z.
+    + s!. firstorder congruence.
+    + s!. eapply in_accum_hatom_in_trms_iff_HC_occurs_in_trms.
+    + destruct c as [hc | cc]; ss!.
+  - clear in_accum_hatom_in_trms_iff_HC_occurs_in_trms; revert hc. trms_ind ts; intros z.
+    + s!. firstorder congruence.
+    + s!. rewrite IH. rewrite in_accum_hatom_in_trm_iff_HC_occurs_in_trm. reflexivity.
+Qed.
+
+Fixpoint accum_hatom_in_frm (p : frm L') : list hatom :=
+  match p with
+  | Rel_frm R ts => accum_hatom_in_trms ts
+  | Eqn_frm t1 t2 => accum_hatom_in_trm t1 ++ accum_hatom_in_trm t2
+  | Neg_frm p1 => accum_hatom_in_frm p1
+  | Imp_frm p1 p2 => accum_hatom_in_frm p1 ++ accum_hatom_in_frm p2
+  | All_frm y p1 => L.remove eq_dec (inl y) (accum_hatom_in_frm p1)
+  end.
+
+Lemma in_accum_hatom_in_frm_iff_is_free_in_frm x (p : frm L')
+  : L.In (inl x) (accum_hatom_in_frm p) <-> is_free_in_frm x p = true.
+Proof.
+  revert x. frm_ind p; i.
+  - simpl. eapply in_accum_hatom_in_trms_iff_is_free_in_trms.
+  - simpl. rewrite orb_true_iff. do 2 rewrite <- in_accum_hatom_in_trm_iff_is_free_in_trm. rewrite L.in_app_iff. reflexivity.
+  - ss!.
+  - ss!.
+  - ss!.
+Qed.
+
+#[local] Hint Rewrite in_accum_hatom_in_trm_iff_HC_occurs_in_trm in_accum_hatom_in_trms_iff_HC_occurs_in_trms : simplication_hints.
+
+Lemma in_accum_hatom_in_frm_iff_HC_occurs_in_frm hc (p : frm L')
+  : L.In (inr hc) (accum_hatom_in_frm p) <-> HC_occurs_in_frm hc p = true.
+Proof.
+  revert hc. frm_ind p; done!.
+Qed.
+
+#[local] Hint Rewrite in_accum_hatom_in_frm_iff_HC_occurs_in_frm : simplication_hints.
+
+Definition hchi_frm (sigma : hsubst) (p : frm L') : ivar :=
+  1 + maxs (L.map (last_ivar_trm ∘ sigma)%prg (accum_hatom_in_frm p)).
+
+Definition nil_hsubst : hsubst :=
+  fun z : hatom =>
+  match z with
+  | inl x => Var_trm x
+  | inr c => @Con_trm L' (inr c)
+  end.
+
+Lemma to_hsubst_nil_subst
+  : forall z, to_hsubst nil_subst z = nil_hsubst z.
+Proof.
+  intros [z | z]; reflexivity.
+Qed.
+
+Definition cons_hsubst (x : hatom) (t : trm L') (sigma : hsubst) : hsubst :=
+  fun z : hatom => if Prelude.eqb z x then t else sigma z.
+
+Lemma to_hsubst_cons_subst (x : ivar) (t : trm L') (s : subst L')
+  : forall z, to_hsubst (cons_subst x t s) z = cons_hsubst (inl x) t (to_hsubst s) z.
+Proof.
+  intros [z | z]; unfold to_hsubst, cons_hsubst, nil_hsubst, cons_subst, nil_subst.
+  - destruct (eq_dec z x) as [EQ | NE], (eqb (inl z) (inl x)) as [ | ] eqn: H_OBS; done!.
+  - destruct (eqb (inr z) (inl x)) as [ | ] eqn: H_OBS; done!.
+Qed.
+
+Definition one_hsubst (x : hatom) (t : trm L') : hsubst :=
+  cons_hsubst x t nil_hsubst.
+
+Lemma to_hsubst_one_subst (x : ivar) (t : trm L')
+  : forall z, to_hsubst (one_subst x t) z = one_hsubst (inl x) t z.
+Proof.
+  intros [z | z]; unfold to_hsubst, one_hsubst, cons_hsubst, nil_hsubst, one_subst, cons_subst, nil_subst.
+  - destruct (eq_dec z x) as [EQ | NE], (eqb (inl z) (inl x)) as [ | ] eqn: H_OBS; done!.
+  - destruct (eqb (inr z) (inl x)) as [ | ] eqn: H_OBS; done!.
+Qed.
+
+Fixpoint hsubst_trm (sigma : hsubst) (t : trm L') : trm L' :=
+  match t with
+  | Var_trm x => sigma (inl x)
+  | Fun_trm f ts => Fun_trm f (hsubst_trms sigma ts)
+  | Con_trm c =>
+    match c with
+    | inl cc => Con_trm c
+    | inr hc => sigma (inr hc)
+    end
+  end
+with hsubst_trms {n : nat} (sigma : hsubst) (ts : trms L' n) : trms L' n :=
+  match ts with
+  | O_trms => O_trms
+  | S_trms n t ts => S_trms n (hsubst_trm sigma t) (hsubst_trms sigma ts)
+  end.
+
+Fixpoint hsubst_frm (sigma : hsubst) (p : frm L') : frm L' :=
+  let chi : ivar := hchi_frm sigma p in
+  match p with
+  | Rel_frm R ts => Rel_frm R (hsubst_trms sigma ts)
+  | Eqn_frm t1 t2 => Eqn_frm (hsubst_trm sigma t1) (hsubst_trm sigma t2)
+  | Neg_frm p1 => Neg_frm (hsubst_frm sigma p1)
+  | Imp_frm p1 p2 => Imp_frm (hsubst_frm sigma p1) (hsubst_frm sigma p2)
+  | All_frm y p1 => All_frm chi (hsubst_frm (cons_hsubst (inl y) (Var_trm chi) sigma) p1)
+  end.
+
+Lemma hsubst_trm_unfold (sigma : hsubst) (t : trm L') :
+  hsubst_trm sigma t =
+  match t with
+  | Var_trm x => sigma (inl x)
+  | Fun_trm f ts => Fun_trm f (hsubst_trms sigma ts)
+  | Con_trm c =>
+    match c with
+    | inl cc => Con_trm c
+    | inr hc => sigma (inr hc)
+    end
+  end.
+Proof.
+  destruct t; reflexivity.
+Defined.
+
+Lemma hsubst_trms_unfold n (sigma : hsubst) (ts : trms L' n) :
+  hsubst_trms sigma ts =
+  match ts with
+  | O_trms => O_trms
+  | S_trms n t ts => S_trms n (hsubst_trm sigma t) (hsubst_trms sigma ts)
+  end.
+Proof.
+  destruct ts; reflexivity.
+Defined.
+
+Lemma hsubst_frm_unfold (sigma : hsubst) (p : frm L') :
+  hsubst_frm sigma p =
+  match p with
+  | Rel_frm R ts => Rel_frm R (hsubst_trms sigma ts)
+  | Eqn_frm t1 t2 => Eqn_frm (hsubst_trm sigma t1) (hsubst_trm sigma t2)
+  | Neg_frm p1 => Neg_frm (hsubst_frm sigma p1)
+  | Imp_frm p1 p2 => Imp_frm (hsubst_frm sigma p1) (hsubst_frm sigma p2)
+  | All_frm y p1 =>
+    let z : ivar := hchi_frm sigma p in
+    All_frm z (hsubst_frm (cons_hsubst (inl y) (Var_trm z) sigma) p1)
+  end.
+Proof.
+  destruct p; reflexivity.
+Defined.
+
+Definition hsubst_compose (sigma : hsubst) (sigma' : hsubst) : hsubst :=
+  fun z : hatom => hsubst_trm sigma' (sigma z).
+
+Fixpoint occurs_free_in_trm (z : hatom) (t : trm L') : bool :=
+  match t with
+  | Var_trm x => Prelude.eqb z (inl x)
+  | Fun_trm f ts => occurs_free_in_trms z ts
+  | Con_trm c =>
+    match c with
+    | inl cc => false
+    | inr hc => Prelude.eqb z (inr hc)
+    end
+  end
+with occurs_free_in_trms {n : nat} (z : hatom) (ts : trms L' n) : bool :=
+  match ts with
+  | O_trms => false
+  | S_trms n t ts => occurs_free_in_trm z t || occurs_free_in_trms z ts
+  end.
+
+Fixpoint occurs_free_in_frm (z : hatom) (p : frm L') : bool :=
+  match p with
+  | Rel_frm R ts => occurs_free_in_trms z ts
+  | Eqn_frm t1 t2 => occurs_free_in_trm z t1 || occurs_free_in_trm z t2
+  | Neg_frm p1 => occurs_free_in_frm z p1
+  | Imp_frm p1 p2 => occurs_free_in_frm z p1 || occurs_free_in_frm z p2
+  | All_frm y p1 => occurs_free_in_frm z p1 && negb (Prelude.eqb z (inl y))
+  end.
+
+Lemma occurs_free_in_trm_unfold (z : hatom) (t : trm L') :
+  occurs_free_in_trm z t =
+  match t with
+  | Var_trm x => Prelude.eqb z (inl x)
+  | Fun_trm f ts => occurs_free_in_trms z ts
+  | Con_trm c =>
+    match c with
+    | inl cc => false
+    | inr hc => Prelude.eqb z (inr hc)
+    end
+  end.
+Proof.
+  destruct t; reflexivity.
+Defined.
+
+Lemma occurs_free_in_trms_unfold n (z : hatom) (ts : trms L' n) :
+  occurs_free_in_trms z ts =
+  match ts with
+  | O_trms => false
+  | S_trms n t ts => occurs_free_in_trm z t || occurs_free_in_trms z ts
+  end.
+Proof.
+  destruct ts; reflexivity.
+Defined.
+
+Lemma occurs_free_in_frm_unfold (z : hatom) (p : frm L') :
+  occurs_free_in_frm z p =
+  match p with
+  | Rel_frm R ts => occurs_free_in_trms z ts
+  | Eqn_frm t1 t2 => occurs_free_in_trm z t1 || occurs_free_in_trm z t2
+  | Neg_frm p1 => occurs_free_in_frm z p1
+  | Imp_frm p1 p2 => occurs_free_in_frm z p1 || occurs_free_in_frm z p2
+  | All_frm y p1 => occurs_free_in_frm z p1 && negb (Prelude.eqb z (inl y))
+  end.
+Proof.
+  destruct p; reflexivity.
+Defined.
+
+Lemma occurs_free_in_trm_iff (z : hatom) (t : trm L')
+  : occurs_free_in_trm z t = true <-> In z (accum_hatom_in_trm t)
+with occurs_free_in_trms_iff n (z : hatom) (ts : trms L' n)
+  : occurs_free_in_trms z ts = true <-> In z (accum_hatom_in_trms ts).
+Proof.
+  - clear occurs_free_in_trm_iff. revert z; trm_ind t; simpl; i.
+    + rewrite eqb_eq. done!.
+    + eapply occurs_free_in_trms_iff.
+    + destruct c as [cc | hc]; simpl.
+      * firstorder congruence.
+      * rewrite eqb_eq. firstorder.
+  - clear occurs_free_in_trms_iff. revert z; trms_ind ts; simpl; i.
+    + done!.
+    + done!.
+Qed.
+
+#[local] Hint Rewrite occurs_free_in_trm_iff occurs_free_in_trms_iff : simplication_hints.
+
+Lemma occurs_free_in_frm_iff (z : hatom) (p : frm L')
+  : occurs_free_in_frm z p = true <-> In z (accum_hatom_in_frm p).
+Proof.
+  revert z. frm_ind p; done!.
+Qed.
+
+Lemma hchi_frm_not_free (sigma : hsubst) (p : frm L') (z : hatom)
+  (OCCURS : occurs_free_in_frm z p = true)
+  : is_free_in_trm (hchi_frm sigma p) (sigma z) = false.
+Proof.
+  eapply last_ivar_trm_gt. unfold hchi_frm.
+  enough (WTS : last_ivar_trm (sigma z) <= maxs (L.map (last_ivar_trm ∘ sigma)%prg (accum_hatom_in_frm p))) by lia.
+  eapply in_maxs_ge. unfold "∘"%prg. eapply in_map_iff.
+  rewrite occurs_free_in_frm_iff in OCCURS. done!.
+Qed.
+
+Definition trm_is_fresh_in_hsubst (x : ivar) (sigma : hsubst) (t : trm L') : bool :=
+  L.forallb (negb ∘ is_free_in_trm x ∘ sigma)%prg (accum_hatom_in_trm t).
+
+Definition trms_is_fresh_in_hsubst {n : nat} (x : ivar) (sigma : hsubst) (ts : trms L' n) : bool :=
+  L.forallb (negb ∘ is_free_in_trm x ∘ sigma)%prg (accum_hatom_in_trms ts).
+
+Definition frm_is_fresh_in_hsubst (x : ivar) (sigma : hsubst) (p : frm L') : bool :=
+  L.forallb (negb ∘ is_free_in_trm x ∘ sigma)%prg (accum_hatom_in_frm p).
+
+Lemma trm_is_fresh_in_hsubst_iff (t : trm L') (z : ivar) (sigma : hsubst)
+  : trm_is_fresh_in_hsubst z sigma t = true <-> is_free_in_trm z (hsubst_trm sigma t) = false
+with trms_is_fresh_in_hsubst_iff n (ts : trms L' n) (z : ivar) (sigma : hsubst)
+  : trms_is_fresh_in_hsubst z sigma ts = true <-> is_free_in_trms z (hsubst_trms sigma ts) = false.
+Proof.
+  - unfold trm_is_fresh_in_hsubst. unfold "∘"%prg. clear trm_is_fresh_in_hsubst_iff. revert z sigma. trm_ind t; simpl; i.
+    + split; intros H; [rewrite andb_true_iff in H; destruct H as [H _]; rewrite negb_true_iff in H; done| rewrite andb_true_iff; split; [rewrite negb_true_iff; done | done]].
+    + eapply trms_is_fresh_in_hsubst_iff.
+    + destruct c as [cc | hc].
+      * ss!. 
+      * simpl. split.
+        { rewrite andb_true_iff. intros [H _]. rewrite negb_true_iff in H. done!. }
+        { rewrite andb_true_iff. rewrite negb_true_iff. done!. }
+  - unfold trms_is_fresh_in_hsubst. clear trms_is_fresh_in_hsubst_iff. revert z sigma. trms_ind ts; simpl; i.
+    + done.
+    + rewrite forallb_app. rewrite is_free_in_trms_unfold. rewrite orb_false_iff. rewrite andb_true_iff. rewrite IH. rewrite <- trm_is_fresh_in_hsubst_iff. reflexivity.
+Qed.
+
+Lemma frm_is_fresh_in_hsubst_iff (p : frm L') (z : ivar) (sigma : hsubst)
+  : frm_is_fresh_in_hsubst z sigma p = true <-> is_free_in_frm z (hsubst_frm sigma p) = false.
+Proof.
+  revert z sigma. unfold frm_is_fresh_in_hsubst. frm_ind p; simpl; ii.
+  - eapply trms_is_fresh_in_hsubst_iff.
+  - rewrite orb_false_iff. do 2 rewrite <- trm_is_fresh_in_hsubst_iff.
+    unfold "∘"%prg. rewrite forallb_app. rewrite andb_true_iff. done.
+  - done.
+  - rewrite forallb_app. rewrite orb_false_iff. rewrite andb_true_iff. rewrite IH1, IH2. done.
+  - split.
+    + intros H_forallb. rewrite andb_false_iff.
+      destruct (z =? hchi_frm sigma (All_frm y p1))%nat as [ | ] eqn : OBS.
+      { simpl. right. done. }
+      { left. rewrite Nat.eqb_neq in OBS. eapply IH1. rewrite forallb_forall.
+        intros x x_in. unfold "∘"%prg. rewrite negb_true_iff. unfold cons_hsubst.
+        unfold Prelude.eqb. destruct (Prelude.eq_dec x (inl y)) as [H_eq | H_ne].
+        - destruct (is_free_in_trm z (Var_trm (hchi_frm sigma (All_frm y p1)))) as [ | ] eqn : EQ.
+          + contradiction OBS. symmetry. subst x. rewrite <- fv_is_free_in_trm in EQ.
+            simpl in EQ. done!.
+          + done!.
+        - rewrite forallb_forall in H_forallb. unfold "∘"%prg in H_forallb.
+          rewrite <- negb_true_iff. eapply H_forallb. eapply L.in_remove_iff. done.
+      }
+    + rewrite andb_false_iff. rewrite negb_false_iff. rewrite Nat.eqb_eq. unfold "∘"%prg in *. intros [NOT_FREE | ->].
+      { eapply IH1 in NOT_FREE. rewrite forallb_forall in NOT_FREE. rewrite forallb_forall.
+        intros x x_in. rewrite negb_true_iff. rewrite L.in_remove_iff in x_in. destruct x_in as [x_in x_ne_y].
+        apply NOT_FREE in x_in. rewrite negb_true_iff in x_in. unfold cons_hsubst in x_in.
+        unfold Prelude.eqb in *. destruct (Prelude.eq_dec x (inl y)) as [H_eq | H_ne]; try done.
+      }
+      { rewrite forallb_forall. intros x x_in. apply L.in_remove_iff in x_in. destruct x_in as [x_in x_ne_y].
+        rewrite negb_true_iff. eapply hchi_frm_not_free. simpl. rewrite andb_true_iff.
+        split; [rewrite <- occurs_free_in_frm_iff in x_in | rewrite negb_true_iff; unfold Prelude.eqb; destruct (eq_dec x (inl y))]; try done.
+      }
+Qed.
+
+Theorem hchi_frm_is_fresh_in_hsubst (p : frm L') (sigma : hsubst)
+  : frm_is_fresh_in_hsubst (hchi_frm sigma p) sigma p = true.
+Proof.
+  unfold frm_is_fresh_in_hsubst. rewrite forallb_forall. ii.
+  unfold "∘"%prg. rewrite negb_true_iff. eapply hchi_frm_not_free.
+  rewrite occurs_free_in_frm_iff. done.
+Qed.
+
+Lemma hchi_frm_nil (p : frm L')
+  : is_free_in_frm (hchi_frm nil_hsubst p) p = false.
+Proof.
+  pose proof (hchi_frm_is_fresh_in_hsubst p nil_hsubst) as claim1.
+  unfold frm_is_fresh_in_hsubst in claim1.
+  rewrite <- not_true_iff_false. intros CONTRA. 
+  rewrite forallb_forall in claim1. unfold "∘"%prg in claim1.
+  rewrite <- in_accum_hatom_in_frm_iff_is_free_in_frm in CONTRA.
+  apply claim1 in CONTRA. rewrite negb_true_iff in CONTRA.
+  unfold nil_hsubst in CONTRA at 2. rewrite is_free_in_trm_unfold in CONTRA.
+  rewrite Nat.eqb_neq in CONTRA. contradiction.
+Qed.
+
+Definition equiv_hsubst_in_frm (sigma1 : hsubst) (sigma2 : hsubst) (p : frm L') : Prop :=
+  forall z : hatom, forall FREE : occurs_free_in_frm z p = true, sigma1 z = sigma2 z.
+
+Theorem hchi_frm_compat_equiv_hsubst (sigma1 : hsubst) (sigma2 : hsubst) (p : frm L')
+  (EQUIV : equiv_hsubst_in_frm sigma1 sigma2 p)
+  : hchi_frm sigma1 p = hchi_frm sigma2 p.
+Proof.
+  unfold hchi_frm. f_equal. eapply maxs_ext. intros n. unfold "∘"%prg.
+  split; intros H_in; eapply in_map_iff; apply in_map_iff in H_in; destruct H_in as [x [<- H_in]].
+  - exists x. rewrite -> EQUIV. try done!.
+    rewrite occurs_free_in_frm_iff. done!.
+  - exists x. rewrite -> EQUIV. try done!.
+    rewrite occurs_free_in_frm_iff. done!.
+Qed.
+
+Lemma equiv_hsubst_in_trm_implies_hsubst_trm_same (sigma1 : hsubst) (sigma2 : hsubst) (t : trm L')
+  (EQUIV : forall z : hatom, forall FREE : occurs_free_in_trm z t = true, sigma1 z = sigma2 z)
+  : hsubst_trm sigma1 t = hsubst_trm sigma2 t
+with equiv_hsubst_in_trms_implies_hsubst_trms_same n (sigma1 : hsubst) (sigma2 : hsubst) (ts : trms L' n)
+  (EQUIV : forall z : hatom, forall FREE : occurs_free_in_trms z ts = true, sigma1 z = sigma2 z)
+  : hsubst_trms sigma1 ts = hsubst_trms sigma2 ts.
+Proof.
+  - clear equiv_hsubst_in_trm_implies_hsubst_trm_same. revert sigma1 sigma2 EQUIV. trm_ind t; simpl; ii.
+    + eapply EQUIV. rewrite eqb_eq. done.
+    + f_equal. eapply equiv_hsubst_in_trms_implies_hsubst_trms_same. exact EQUIV.
+    + destruct c as [cc | hc].
+      * reflexivity.
+      * eapply EQUIV. rewrite eqb_eq. done!.
+  - clear equiv_hsubst_in_trms_implies_hsubst_trms_same. revert sigma1 sigma2 EQUIV. trms_ind ts; simpl; ii.
+    + reflexivity.
+    + f_equal.
+      * eapply equiv_hsubst_in_trm_implies_hsubst_trm_same. ii. eapply EQUIV. rewrite orb_true_iff. left. exact FREE.
+      * eapply IH. ii. eapply EQUIV. rewrite orb_true_iff. right. exact FREE.
+Qed.
+
+Lemma equiv_hsubst_in_frm_implies_hsubst_frm_same (sigma1 : hsubst) (sigma2 : hsubst) (p : frm L')
+  (EQUIV : equiv_hsubst_in_frm sigma1 sigma2 p)
+  : hsubst_frm sigma1 p = hsubst_frm sigma2 p.
+Proof.
+  revert sigma1 sigma2 EQUIV. unfold equiv_hsubst_in_frm. frm_ind p; simpl; ii.
+  - simpl in EQUIV. f_equal.
+    eapply equiv_hsubst_in_trms_implies_hsubst_trms_same. done.
+  - simpl in EQUIV. f_equal.
+    + eapply equiv_hsubst_in_trm_implies_hsubst_trm_same. ii.
+      eapply EQUIV. rewrite orb_true_iff. done!.
+    + eapply equiv_hsubst_in_trm_implies_hsubst_trm_same. ii.
+      eapply EQUIV. rewrite orb_true_iff. done!.
+  - f_equal. eapply IH1. done.
+  - f_equal.
+    + eapply IH1. ii. eapply EQUIV. rewrite orb_true_iff. done!.
+    + eapply IH2. ii. eapply EQUIV. rewrite orb_true_iff. done!.
+  - f_equal.
+    + eapply hchi_frm_compat_equiv_hsubst. unfold equiv_hsubst_in_frm. simpl. done.
+    + eapply IH1. ii. unfold cons_hsubst. unfold eqb in *. destruct (eq_dec z (inl y)) as [H_yes | H_no].
+      { f_equal. subst z. eapply hchi_frm_compat_equiv_hsubst. unfold equiv_hsubst_in_frm. simpl. done. }
+      { eapply EQUIV. rewrite andb_true_iff. split. done. eapply negb_true_iff. unfold Prelude.eqb. destruct (eq_dec z (inl y)); done. }
+Qed.
+
+Lemma distr_hcompose_one (sigma1 : hsubst) (sigma2 : hsubst) (x : hatom) (y : ivar) (z : hatom) (t : trm L') (p : frm L')
+  (FRESH : forallb (negb ∘ occurs_free_in_trm (inl y) ∘ sigma1)%prg (remove eq_dec x (accum_hatom_in_frm p)) = true)
+  (FREE : occurs_free_in_frm z p = true)
+  : cons_hsubst x t (hsubst_compose sigma1 sigma2) z = hsubst_compose (cons_hsubst x (Var_trm y) sigma1) (cons_hsubst (inl y) t sigma2) z.
+Proof.
+  unfold hsubst_compose, cons_hsubst. unfold Prelude.eqb. destruct (eq_dec z x) as [H_eq | H_ne].
+  - subst z. simpl. destruct (eq_dec (inl y) (inl y)); done.
+  - rewrite forallb_forall in FRESH. unfold "∘"%prg in FRESH.
+    assert (NOT_FREE : occurs_free_in_trm (inl y) (sigma1 z) = false).
+    { rewrite <- negb_true_iff. eapply FRESH. rewrite L.in_remove_iff. rewrite <- occurs_free_in_frm_iff. done!. }
+    eapply equiv_hsubst_in_trm_implies_hsubst_trm_same. intros z' FREE'. destruct (eq_dec z' (inl y)) as [EQ | NE]; try done!.
+Qed.
+
+#[local] Tactic Notation "done" :=
+  first [now firstorder | done!].
+
+Definition occurs_free_in_trm_wrt (z : hatom) (sigma : hsubst) (t : trm L') : Prop :=
+  exists x : hatom, occurs_free_in_trm x t = true /\ occurs_free_in_trm z (sigma x) = true.
+
+Definition occurs_free_in_trms_wrt {n : nat} (z : hatom) (sigma : hsubst) (ts : trms L' n) : Prop :=
+  exists x : hatom, occurs_free_in_trms x ts = true /\ occurs_free_in_trm z (sigma x) = true.
+
+Definition occurs_free_in_frm_wrt (z : hatom) (sigma : hsubst) (p : frm L') : Prop :=
+  exists x : hatom, occurs_free_in_frm x p = true /\ occurs_free_in_trm z (sigma x) = true.
+
+Fixpoint occurs_free_in_trm_wrt_iff (t : trm L') (z : hatom) (sigma : hsubst) {struct t}
+  : occurs_free_in_trm_wrt z sigma t <-> occurs_free_in_trm z (hsubst_trm sigma t) = true
+with occurs_free_in_trms_wrt_iff n (ts : trms L' n) (z : hatom) (sigma : hsubst) {struct ts}
+  : occurs_free_in_trms_wrt z sigma ts <-> occurs_free_in_trms z (hsubst_trms sigma ts) = true.
+Proof.
+  - clear occurs_free_in_trm_wrt_iff. destruct t as [x | f ts | [cc | hc]]; simpl; i.
+    + clear occurs_free_in_trms_wrt_iff. split.
+      * intros [y [FREE FREE']]. unfold Prelude.eqb in FREE. destruct (eq_dec y (inl x)); done.
+      * unfold occurs_free_in_trm_wrt. intros FREE. exists (inl x). simpl. rewrite eqb_eq. done.
+    + pose proof (occurs_free_in_trms_wrt_iff (L.(function_arity_table) f) ts z sigma) as H. clear occurs_free_in_trms_wrt_iff. split.
+      * intros [y [FREE FREE']]. done.
+      * intros FREE. done.
+    + clear occurs_free_in_trms_wrt_iff. done.
+    + clear occurs_free_in_trms_wrt_iff. split.
+      * intros [y [FREE FREE']]. unfold Prelude.eqb in FREE. destruct (eq_dec y (inr hc)); done.
+      * unfold occurs_free_in_trm_wrt. intros FREE. exists (inr hc). simpl. rewrite eqb_eq. split; trivial.
+  - destruct ts as [ | n t ts]; simpl; i.
+    + clear occurs_free_in_trm_wrt_iff occurs_free_in_trms_wrt_iff. done.
+    + pose proof (occurs_free_in_trm_wrt_iff t z sigma) as H. clear occurs_free_in_trm_wrt_iff. pose proof (occurs_free_in_trms_wrt_iff n ts z sigma) as H'. clear occurs_free_in_trms_wrt_iff. split.
+      * intros [x [FREE FREE']]. rewrite orb_true_iff. simpl in FREE. rewrite orb_true_iff in FREE. destruct FREE as [FREE | FREE].
+        { left. rewrite <- H. exists x. split; trivial. }
+        { right. rewrite <- H'. exists x. split; trivial. }
+      * rewrite orb_true_iff. intros [FREE | FREE].
+        { rewrite <- H in FREE. destruct FREE as [x [FREE FREE']]. exists x. simpl. rewrite orb_true_iff. split; [left; exact FREE | exact FREE']. }
+        { rewrite <- H' in FREE. destruct FREE as [x [FREE FREE']]. exists x. simpl. rewrite orb_true_iff. split; [right; exact FREE | exact FREE']. }
+Qed.
+
+Lemma occurs_free_in_frm_wrt_iff (p : frm L') (z : hatom) (sigma : hsubst)
+  : occurs_free_in_frm_wrt z sigma p <-> occurs_free_in_frm z (hsubst_frm sigma p) = true.
+Proof.
+  revert z sigma. unfold occurs_free_in_frm_wrt. frm_ind p; simpl; i.
+  - split.
+    + intros [y [FREE FREE']]. eapply occurs_free_in_trms_wrt_iff. done.
+    + intros FREE. apply occurs_free_in_trms_wrt_iff in FREE. done.
+  - split.
+    + intros [y [FREE FREE']]. rewrite orb_true_iff in FREE. rewrite orb_true_iff. destruct FREE as [FREE | FREE].
+      * left. eapply occurs_free_in_trm_wrt_iff. done.
+      * right. eapply occurs_free_in_trm_wrt_iff. done.
+    + intros FREE. rewrite orb_true_iff in FREE. destruct FREE as [FREE | FREE].
+      * apply occurs_free_in_trm_wrt_iff in FREE. destruct FREE as [y [FREE FREE']].
+        exists y. rewrite orb_true_iff. done.
+      * apply occurs_free_in_trm_wrt_iff in FREE. destruct FREE as [y [FREE FREE']].
+        exists y. rewrite orb_true_iff. done.
+  - done.
+  - split.
+    + intros [y [FREE FREE']]. rewrite orb_true_iff in FREE. rewrite orb_true_iff. destruct FREE as [FREE | FREE].
+      * left. eapply IH1. done.
+      * right. eapply IH2. done.
+    + intros FREE. rewrite orb_true_iff in FREE. destruct FREE as [FREE | FREE].
+      * apply IH1 in FREE. destruct FREE as [y [FREE FREE']].
+        exists y. rewrite orb_true_iff. done.
+      * apply IH2 in FREE. destruct FREE as [y [FREE FREE']].
+        exists y. rewrite orb_true_iff. done.
+  - split.
+    + intros [w [FREE FREE']]. rewrite andb_true_iff in FREE. rewrite negb_true_iff in FREE. rewrite eqb_neq in FREE.
+      destruct FREE as [FREE w_ne_y]. rewrite andb_true_iff. rewrite negb_true_iff. split.
+      * eapply IH1. exists w. split; trivial. unfold cons_hsubst.
+        unfold Prelude.eqb. destruct (eq_dec w (inl y)) as [EQ | NE]; done.
+      * rewrite eqb_neq. intros CONTRA.
+        assert (claim1 : frm_is_fresh_in_hsubst (hchi_frm sigma (All_frm y p1)) sigma (All_frm y p1) = true).
+        { exact (hchi_frm_is_fresh_in_hsubst (All_frm y p1) sigma). }
+        unfold frm_is_fresh_in_hsubst in claim1. rewrite forallb_forall in claim1.
+        assert (claim2 : In w (accum_hatom_in_frm (All_frm y p1))).
+        { rewrite <- occurs_free_in_frm_iff. simpl. rewrite andb_true_iff. rewrite negb_true_iff. rewrite eqb_neq. done. }
+        apply claim1 in claim2. unfold "∘"%prg in claim2. rewrite negb_true_iff in claim2.
+        subst z. rewrite occurs_free_in_trm_iff in FREE'. rewrite in_accum_hatom_in_trm_iff_is_free_in_trm in FREE'. done.
+    + rewrite andb_true_iff. rewrite negb_true_iff. rewrite eqb_neq.
+      set (w := hchi_frm sigma (All_frm y p1)). intros [FREE NE].
+      apply IH1 in FREE. destruct FREE as [x [FREE FREE']].
+      unfold cons_hsubst in FREE'. unfold eqb in FREE'. destruct (eq_dec x (inl y)) as [x_eq_y | x_ne_y].
+      * subst x. contradiction NE. apply occurs_free_in_trm_iff in FREE'. simpl in FREE'. done.
+      * exists x. rewrite andb_true_iff. rewrite negb_true_iff. rewrite eqb_neq. done.
+Qed.
+
+Lemma hchi_frm_ext (sigma1 : hsubst) (sigma2 : hsubst) (p1 : frm L') (p2 : frm L')
+  (EQUIV : forall z : hatom, occurs_free_in_frm_wrt z sigma1 p1 <-> occurs_free_in_frm_wrt z sigma2 p2)
+  : hchi_frm sigma1 p1 = hchi_frm sigma2 p2.
+Proof.
+  assert (ENOUGH : forall xs : list hatom, forall f : hatom -> list ivar, maxs (L.map (maxs ∘ f)%prg xs) = maxs (L.flat_map f xs)).
+  { induction xs; simpl; i; eauto. unfold "∘"%prg. rewrite maxs_app. f_equal. eauto. }
+  unfold hchi_frm. f_equal. unfold last_ivar_trm.
+  change (maxs (L.map (maxs ∘ (fvs_trm ∘ sigma1))%prg (accum_hatom_in_frm p1)) = maxs (L.map (maxs ∘ (fvs_trm ∘ sigma2))%prg (accum_hatom_in_frm p2))).
+  do 2 rewrite ENOUGH. eapply maxs_ext. intros z. do 2 rewrite in_flat_map.
+  unfold "∘"%prg. split; intros (y&IN&IN').
+  - assert (claim : occurs_free_in_frm_wrt (inl z) sigma1 p1).
+    { exists y. split.
+      - rewrite occurs_free_in_frm_iff; trivial.
+      - rewrite occurs_free_in_trm_iff, in_accum_hatom_in_trm_iff_is_free_in_trm; done.
+    }
+    rewrite -> EQUIV in claim. destruct claim as (x&OCCURS&OCCURS'). exists x. split.
+    + rewrite occurs_free_in_frm_iff in OCCURS. done.
+    + rewrite fv_is_free_in_trm, <- in_accum_hatom_in_trm_iff_is_free_in_trm, <- occurs_free_in_trm_iff. done.
+  - assert (claim : occurs_free_in_frm_wrt (inl z) sigma2 p2).
+    { exists y. split.
+      - rewrite occurs_free_in_frm_iff; trivial.
+      - rewrite occurs_free_in_trm_iff, in_accum_hatom_in_trm_iff_is_free_in_trm; done.
+    }
+    rewrite <- EQUIV in claim. destruct claim as (x&OCCURS&OCCURS'). exists x. split.
+    + rewrite occurs_free_in_frm_iff in OCCURS. done.
+    + rewrite fv_is_free_in_trm, <- in_accum_hatom_in_trm_iff_is_free_in_trm, <- occurs_free_in_trm_iff. done.
+Qed.
+
+Theorem hsubst_compose_trm_spec (t : trm L') (sigma : hsubst) (sigma': hsubst)
+  : hsubst_trm (hsubst_compose sigma sigma') t = hsubst_trm sigma' (hsubst_trm sigma t)
+with hsubst_compose_trms_spec n (ts : trms L' n) (sigma : hsubst) (sigma': hsubst)
+  : hsubst_trms (hsubst_compose sigma sigma') ts = hsubst_trms sigma' (hsubst_trms sigma ts).
+Proof.
+  - revert sigma sigma'. trm_ind t; simpl; i.
+    + done.
+    + f_equal. eapply hsubst_compose_trms_spec.
+    + destruct c as [cc | hc]; done.
+  - revert sigma sigma'. trms_ind ts; simpl; i.
+    + done.
+    + f_equal.
+      * eapply hsubst_compose_trm_spec.
+      * eapply IH.
+Qed.
+
+Theorem hsubst_compose_frm_spec (p : frm L') (sigma : hsubst) (sigma': hsubst)
+  : hsubst_frm (hsubst_compose sigma sigma') p = hsubst_frm sigma' (hsubst_frm sigma p).
+Proof.
+  revert sigma sigma'. frm_ind p; simpl; i.
+  - f_equal; eapply hsubst_compose_trms_spec.
+  - f_equal; eapply hsubst_compose_trm_spec.
+  - done.
+  - done.
+  - enough (ENOUGH : hchi_frm sigma' (hsubst_frm sigma (All_frm y p1)) = hchi_frm (hsubst_compose sigma sigma') (All_frm y p1)).
+    { revert ENOUGH.
+      set (x := hchi_frm sigma (All_frm y p1)).
+      set (z := hchi_frm (hsubst_compose sigma sigma') (All_frm y p1)).
+      set (w := hchi_frm sigma' (All_frm x (hsubst_frm (cons_hsubst (inl y) (Var_trm x) sigma) p1))).
+      i. rewrite <- IH1. assert (EQ: z = w) by done. subst z. f_equal; trivial.
+      eapply equiv_hsubst_in_frm_implies_hsubst_frm_same.
+      unfold equiv_hsubst_in_frm. ii.
+      rewrite <- distr_hcompose_one with (p := p1).
+      - done.
+      - pose proof (claim1 := hchi_frm_is_fresh_in_hsubst). unfold frm_is_fresh_in_hsubst in claim1.
+        eapply forallb_forall. intros u u_in. rewrite L.in_remove_iff in u_in. destruct u_in as [u_in NE].
+        unfold "∘"%prg. rewrite negb_true_iff.
+        enough (WTS : occurs_free_in_trm (inl x) (sigma u) <> true) by now destruct (occurs_free_in_trm (inl x) (sigma u)).
+        intros CONTRA. rewrite occurs_free_in_trm_iff in CONTRA. rewrite in_accum_hatom_in_trm_iff_is_free_in_trm in CONTRA.
+        specialize claim1 with (p := All_frm y p1) (sigma := sigma). unfold "∘"%prg in claim1. rewrite forallb_forall in claim1.
+        assert (claim2: In u (accum_hatom_in_frm (All_frm y p1))).
+        { simpl. rewrite L.in_remove_iff. done. }
+        apply claim1 in claim2. rewrite negb_true_iff in claim2. done.
+      - done.
+    }
+    eapply hchi_frm_ext. intros z. split.
+    + simpl. unfold occurs_free_in_frm_wrt. intros [x [FREE FREE']]. simpl in FREE.
+      rewrite andb_true_iff in FREE. rewrite negb_true_iff in FREE. rewrite eqb_neq in FREE.
+      destruct FREE as [FREE NE]. apply occurs_free_in_frm_wrt_iff in FREE. unfold free_in_frm_wrt in FREE.
+      destruct FREE as [w [FREE1 FREE2]]. unfold cons_hsubst in FREE2. unfold eqb in FREE2. destruct (eq_dec w (inl y)) as [w_eq_y | w_ne_y].
+      * unfold occurs_free_in_trm in FREE2. rewrite eqb_eq in FREE2. subst. done.
+      * exists w. simpl. rewrite andb_true_iff. rewrite negb_true_iff. rewrite eqb_neq. split; try tauto.
+        eapply occurs_free_in_trm_wrt_iff. done.
+    + intros [x [FREE FREE']]. simpl in FREE. rewrite andb_true_iff in FREE. rewrite negb_true_iff in FREE. rewrite eqb_neq in FREE. destruct FREE as [FREE NE].
+      apply occurs_free_in_trm_wrt_iff in FREE'. destruct FREE' as [u [FREE' FREE'']]. exists u. split.
+      * eapply occurs_free_in_frm_wrt_iff. exists x. simpl. rewrite andb_true_iff. rewrite negb_true_iff. rewrite eqb_neq. done.
+      * done.
+Qed.
+
+Lemma hcompose_one_hsubst_frm (x1 : hatom) (t1 : trm L') (sigma : hsubst) (p : frm L')
+  : hsubst_frm sigma (hsubst_frm (one_hsubst x1 t1) p) = hsubst_frm (cons_hsubst x1 (hsubst_trm sigma t1) sigma) p.
+Proof.
+  unfold one_hsubst. rewrite <- hsubst_compose_frm_spec. eapply equiv_hsubst_in_frm_implies_hsubst_frm_same. ii.
+  unfold cons_hsubst, hsubst_compose, eqb. destruct (eq_dec z x1) as [z_eq_x1 | z_ne_x1]; try done.
+  unfold nil_hsubst. destruct z; try done.
+Qed.
+
+Lemma cons_hsubst_hsubst_frm (x1 : hatom) (t1 : trm L') (y : hatom) (p : frm L') (sigma : hsubst)
+  (NOT_FREE : occurs_free_in_frm y p = false \/ y = x1)
+  : hsubst_frm (cons_hsubst x1 t1 sigma) p = hsubst_frm (cons_hsubst y t1 sigma) (hsubst_frm (one_hsubst x1 (nil_hsubst y)) p).
+Proof.
+  unfold one_hsubst. rewrite <- hsubst_compose_frm_spec. eapply equiv_hsubst_in_frm_implies_hsubst_frm_same.
+  ii. unfold cons_hsubst, hsubst_compose, eqb. destruct (eq_dec z x1) as [z_eq_x1 | z_ne_x1].
+  - subst z. unfold nil_hsubst. destruct y as [x | c]; simpl.
+    + destruct (eq_dec (inl x) (inl x)); try done.
+    + destruct (eq_dec (inr c) (inr c)); try done.
+  - destruct z as [x | c]; simpl.
+    + destruct (eq_dec (inl x) y) as [z_eq_y | z_ne_y]; try done.
+    + destruct (eq_dec (inr c) y) as [z_eq_y | z_ne_y]; try done.
+Qed.
+
+Lemma nil_hsubst_trm (t : trm L')
+  : hsubst_trm nil_hsubst t = t
+with nil_hsubst_trms n (ts : trms L' n)
+  : hsubst_trms nil_hsubst ts = ts.
+Proof.
+  - clear nil_hsubst_trm. trm_ind t; simpl.
+    + reflexivity.
+    + f_equal. eapply nil_hsubst_trms.
+    + destruct c as [cc | hc]; reflexivity.
+  - clear nil_hsubst_trms. trms_ind ts; simpl.
+    + reflexivity.
+    + f_equal.
+      * eapply nil_hsubst_trm.
+      * eapply IH.
+Qed.
+
+Lemma trivial_hsubst (x : hatom) (p : frm L')
+  : hsubst_frm (one_hsubst x (nil_hsubst x)) p = hsubst_frm nil_hsubst p.
+Proof.
+  eapply equiv_hsubst_in_frm_implies_hsubst_frm_same. ii. unfold one_hsubst, cons_hsubst.
+  unfold eqb. destruct (eq_dec z x); try done.
+Qed.
+
+Theorem subst_hsubst_compat_in_trm (s : subst L') (sigma : hsubst) (t : trm L')
+  (SIM : forall z : hatom, to_hsubst s z = sigma z)
+  : subst_trm s t = hsubst_trm sigma t
+with subst_hsubst_compat_in_trms n (s : subst L') (sigma : hsubst) (ts : trms L' n)
+  (SIM : forall z : hatom, to_hsubst s z = sigma z)
+  : subst_trms s ts = hsubst_trms sigma ts.
+Proof.
+  - clear subst_hsubst_compat_in_trm. revert s sigma SIM. trm_ind t; simpl; i.
+    + rewrite subst_trm_unfold. exact (SIM (inl x)).
+    + rewrite <- subst_hsubst_compat_in_trms with (s := s); trivial.
+    + destruct c as [cc | hc]; [reflexivity | exact (SIM (inr hc))].
+  - clear subst_hsubst_compat_in_trms. revert s sigma SIM. trms_ind ts; simpl; i.
+    + reflexivity.
+    + rewrite <- subst_hsubst_compat_in_trm with (s := s); trivial. rewrite <- IH with (s := s); trivial.
+Qed.
+
+Theorem subst_hsubst_compat_in_frm (s : subst L') (sigma : hsubst) (p : frm L')
+  (SIM : forall z : hatom, to_hsubst s z = sigma z)
+  : subst_frm s p = hsubst_frm sigma p.
+Proof.
+  revert s sigma SIM. revert p.
+  assert (LEMMA : forall A : Set, forall xs : list A, forall f: A -> list ivar, maxs (L.map (maxs ∘ f)%prg xs) = maxs (L.flat_map f xs)).
+  { intros A. induction xs; simpl; i; eauto. unfold "∘"%prg. rewrite maxs_app. f_equal. eauto. }
+  frm_ind p; simpl; i.
+  - f_equal. eapply subst_hsubst_compat_in_trms. done.
+  - f_equal; eapply subst_hsubst_compat_in_trm; done.
+  - f_equal. done.
+  - f_equal; done.
+  - assert (claim : chi_frm s (All_frm y p1) = hchi_frm sigma (All_frm y p1)).
+    { unfold hchi_frm, chi_frm. f_equal.
+      change (maxs (L.map (maxs ∘ (fvs_trm ∘ s))%prg (fvs_frm (All_frm y p1))) = maxs (L.map (maxs ∘ (fvs_trm ∘ sigma))%prg (accum_hatom_in_frm (All_frm y p1)))).
+      do 2 rewrite LEMMA. eapply maxs_ext. intros z. do 2 rewrite in_flat_map. unfold "∘"%prg.
+      split; intros (x&IN&IN').
+      - rewrite fv_is_free_in_frm in IN. simpl in IN. rewrite andb_true_iff, negb_true_iff, Nat.eqb_neq in IN. destruct IN as [IN NE].
+        specialize SIM with (z := inl x). simpl in SIM.
+        exists (inl x). rewrite <- SIM. split; trivial.
+        rewrite in_accum_hatom_in_frm_iff_is_free_in_frm. done.
+      - destruct x as [x | c].
+        + rewrite in_accum_hatom_in_frm_iff_is_free_in_frm in IN. specialize SIM with (z := inl x). simpl in SIM.
+          exists x. rewrite SIM. split; done.
+        + specialize SIM with (z := inr c). simpl in SIM.
+          rewrite <- SIM in IN'. simpl in IN'. done. 
+    }
+    f_equal; trivial. rewrite claim. eapply IH1. intros [x | c]; simpl.
+    + unfold cons_hsubst, cons_subst. destruct (eqb (inl x) (inl y)) as [ | ] eqn : H_OBS.
+      { rewrite eqb_eq in H_OBS. inv H_OBS. destruct (eq_dec y y); try done. }
+      { rewrite eqb_neq in H_OBS. destruct (eq_dec x y); try done. eapply SIM with (z := inl x). }
+    + unfold cons_hsubst, cons_subst. unfold eqb.
+      destruct (eq_dec (inr c) (inl y)) as [EQ | NE].
+      { inv EQ. }
+      { eapply SIM with (z := inr c). }
+Qed.
+
+Definition replace_constant_in_trm (c : Henkin_constants) (ct : trm L') (t : trm L') : trm L' :=
+  hsubst_trm (one_hsubst (inr c) ct) t.
+
+Definition replace_constant_in_trms {n : nat} (c : Henkin_constants) (ct : trm L') (ts : trms L' n) : trms L' n :=
+  hsubst_trms (one_hsubst (inr c) ct) ts.
+
+Definition replace_constant_in_frm (c : Henkin_constants) (ct : trm L') (p : frm L') : frm L' :=
+  hsubst_frm (one_hsubst (inr c) ct) p.
+
+Theorem replace_constant_in_frm_compat_subst (c : Henkin_constants) (ct : trm L') (s : subst L') (p : frm L')
+  (FRESH : forall x : ivar, is_free_in_trm x ct = true -> hsubst_trm (one_hsubst (inr c) ct) (s x) = Var_trm x)
+  : replace_constant_in_frm c ct (subst_frm s p) = subst_frm (replace_constant_in_trm c ct ∘ s)%prg (replace_constant_in_frm c ct p).
+Proof.
+  unfold replace_constant_in_frm at 2. symmetry. erewrite subst_hsubst_compat_in_frm. 2:{ ii. reflexivity. }
+  rewrite <- hsubst_compose_frm_spec. unfold replace_constant_in_frm.
+  erewrite subst_hsubst_compat_in_frm. 2:{ ii. reflexivity. }
+  rewrite <- hsubst_compose_frm_spec. eapply equiv_hsubst_in_frm_implies_hsubst_frm_same.
+  ii. unfold hsubst_compose. unfold "∘"%prg. destruct z as [x | c'].
+  - unfold one_hsubst. simpl. unfold replace_constant_in_trm. reflexivity.
+  - unfold one_hsubst. simpl. unfold cons_hsubst, nil_hsubst.
+    destruct (Prelude.eqb (inr c') (inr c)) as [ | ] eqn : H_OBS.
+    + rewrite eqb_eq in H_OBS. inv H_OBS. unfold replace_constant_in_trm.
+      rewrite <- nil_hsubst_trm. eapply equiv_hsubst_in_trm_implies_hsubst_trm_same.
+      intros [x | c'] OCCURS.
+      * apply occurs_free_in_trm_iff, in_accum_hatom_in_trm_iff_is_free_in_trm, fv_is_free_in_trm in OCCURS. simpl. eapply FRESH. done.
+      * done.
+    + simpl. reflexivity.
+Qed.
+
+Theorem replace_constant_with_fresh_ivar_in_frm (c : Henkin_constants) (s : subst L') (p : frm L') (z : ivar)
+  (FRESH : s z = Var_trm z)
+  : replace_constant_in_frm c (Var_trm z) (subst_frm s p) = subst_frm (replace_constant_in_trm c (Var_trm z) ∘ s)%prg (replace_constant_in_frm c (Var_trm z) p).
+Proof.
+  eapply replace_constant_in_frm_compat_subst. intros x FREE.
+  rewrite is_free_in_trm_unfold in FREE. rewrite Nat.eqb_eq in FREE. subst z.
+  now rewrite FRESH.
+Qed.
+
+Lemma quick_draw_constant (c : Henkin_constants) (x : ivar) (t : trm L') (y : ivar) (p : frm L')
+  (NE : y <> x)
+  : replace_constant_in_frm c (Var_trm y) (subst_frm (one_subst x t) p) = subst_frm (one_subst x (replace_constant_in_trm c (Var_trm y) t)) (replace_constant_in_frm c (Var_trm y) p).
+Proof.
+  rewrite replace_constant_in_frm_compat_subst.
+  - eapply equiv_subst_in_frm_implies_subst_frm_same. unfold "∘"%prg. ii.
+    unfold replace_constant_in_trm, one_hsubst, one_subst, cons_hsubst, cons_subst.
+    destruct (eq_dec z x); try done.
+  - intros z FREE. apply fv_is_free_in_trm in FREE. simpl in FREE. destruct FREE as [-> | []].
+    unfold one_subst, nil_subst, cons_subst. unfold one_hsubst, cons_hsubst, nil_hsubst.
+    destruct (eq_dec z x); try done.
+Qed.
+
+End HSUBST.
+
+Section SIM.
+
+#[local]
+Instance constant_symbols_similarity_instance : Similarity L.(constant_symbols) L'.(constant_symbols) :=
+  fun c : L.(constant_symbols) => fun c' : L'.(constant_symbols) => inl c = c'.
+
+#[local] Existing Instance trm_similarity_instance.
+
+#[local] Existing Instance trms_similarity_instance.
+
+#[local] Existing Instance frm_similarity_instance.
+
+#[local]
+Instance subst_similarity_instance : Similarity (subst L) (subst L') :=
+  fun s : subst L => fun s' : subst L' => forall z : ivar, s z =~= s' z.
+
+Lemma fvs_trm_similarity (t : trm L) (t' : trm L')
+  (t_SIM : t =~= t')
+  : fvs_trm t = fvs_trm t'
+with fvs_trms_similarity n (ts : trms L n) (ts' : trms L' n)
+  (ts_SIM : ts =~= ts')
+  : fvs_trms ts = fvs_trms ts'.
+Proof.
+  - induction t_SIM.
+    + reflexivity.
+    + do 2 rewrite fvs_trm_unfold with (t := Fun_trm _ _). eapply fvs_trms_similarity. exact ts_SIM.
+    + reflexivity.
+  - induction ts_SIM.
+    + reflexivity.
+    + do 2 rewrite fvs_trms_unfold with (ts := S_trms _ _ _). f_equal.
+      * eapply fvs_trm_similarity; exact t_SIM.
+      * eapply IHts_SIM; exact ts_SIM.
+Qed.
+
+#[local] Hint Resolve fvs_trm_similarity fvs_trms_similarity : core.
+
+Lemma fvs_frm_similarity (p : frm L) (p' : frm L')
+  (p_SIM : p =~= p')
+  : fvs_frm p = fvs_frm p'.
+Proof.
+  induction p_SIM; simpl; f_equal; eauto with *.
+Qed.
+
+#[local] Hint Resolve fvs_frm_similarity : core.
+
+Lemma chi_frm_similarity (s : subst L) (s' : subst L') (p : frm L) (p' : frm L')
+  (s_SIM : s =~= s')
+  (p_SIM : p =~= p')
+  : chi_frm s p = chi_frm s' p'.
+Proof with eauto.
+  assert (ENOUGH : forall xs : list ivar, forall f : ivar -> list ivar, maxs (L.map (maxs ∘ f)%prg xs) = maxs (L.flat_map f xs)).
+  { induction xs; simpl; i; eauto. unfold "∘"%prg. rewrite maxs_app. f_equal. eauto. }
+  unfold chi_frm. f_equal. unfold last_ivar_trm.
+  change (maxs (L.map (maxs ∘ (fvs_trm ∘ s))%prg (fvs_frm p)) = maxs (L.map (maxs ∘ (fvs_trm ∘ s'))%prg (fvs_frm p'))).
+  do 2 rewrite ENOUGH. eapply maxs_ext. intros z. do 2 rewrite in_flat_map. unfold "∘"%prg. clear ENOUGH.
+  split; intros [x [FREE FREE']]; exists x; split.
+  - erewrite <- fvs_frm_similarity...
+  - erewrite <- fvs_trm_similarity...
+  - erewrite -> fvs_frm_similarity...
+  - erewrite -> fvs_trm_similarity...
+Qed.
+
+Lemma subst_trm_similiarity (s : subst L) (s' : subst L') (t : trm L) (t' : trm L')
+  (s_SIM : s =~= s')
+  (t_SIM : t =~= t')
+  : subst_trm s t =~= subst_trm s' t'
+with subst_trms_similiarity n (s : subst L) (s' : subst L') (ts : trms L n) (ts' : trms L' n)
+  (s_SIM : s =~= s')
+  (ts_SIM : ts =~= ts')
+  : subst_trms s ts =~= subst_trms s' ts'.
+Proof.
+  - induction t_SIM.
+    + exact (s_SIM x).
+    + do 2 rewrite subst_trm_unfold. econs. eapply subst_trms_similiarity; [exact s_SIM | exact ts_SIM].
+    + do 2 rewrite subst_trm_unfold. econs. exact c_SIM.
+  - induction ts_SIM.
+    + econs.
+    + do 2 rewrite subst_trms_unfold with (ts := S_trms _ _ _). econs.
+      * eapply subst_trm_similiarity; [exact s_SIM | exact t_SIM].
+      * assumption.
+Qed.
+
+Lemma subst_frm_similarity (s : subst L) (s' : subst L') (p : frm L) (p' : frm L')
+  (s_SIM : s =~= s')
+  (p_SIM : p =~= p')
+  : subst_frm s p =~= subst_frm s' p'.
+Proof.
+  revert s s' s_SIM. induction p_SIM; i.
+  - do 2 rewrite subst_frm_unfold. simpl. econs. eapply subst_trms_similiarity; trivial.
+  - do 2 rewrite subst_frm_unfold. simpl. econs; eapply subst_trm_similiarity; trivial.
+  - simpl. econs. done!.
+  - simpl. econs; done!.
+  - assert (claim : (chi_frm s (All_frm y p1)) = (chi_frm s' (All_frm y p1'))).
+    { eapply chi_frm_similarity; trivial. econs; trivial. }
+    simpl. rewrite claim. econs. rewrite <- claim at 1. eapply IHp_SIM.
+    intros z. unfold cons_subst. destruct (eq_dec z y) as [EQ1 | NE1].
+    + rewrite claim. econs.
+    + exact (s_SIM z).
+Qed.
+
+End SIM.
+
+Section TWILIGHT.
+
+Definition twilight (sigma : hsubst) : subst L' :=
+  fun z : ivar => sigma (enum (isEnumerable := @sum_isEnumerable ivar Henkin_constants nat_isEnumerable nat_isEnumerable) z).
+
+Fixpoint twilight_trm (t : trm L') : trm L' :=
+  match t with
+  | Var_trm x => Var_trm (x * 2)
+  | Fun_trm f ts => Fun_trm f (twilight_trms ts)
+  | Con_trm c =>
+    match c with
+    | inl cc => Con_trm c
+    | inr hc => Var_trm (hc * 2 + 1)
+    end
+  end
+with twilight_trms {n : nat} (ts : trms L' n) : trms L' n :=
+  match ts with
+  | O_trms => O_trms
+  | S_trms n t ts => S_trms n (twilight_trm t) (twilight_trms ts)
+  end.
+
+Lemma twilight_trm_unfold (t : trm L') :
+  twilight_trm t =
+  match t with
+  | Var_trm x => Var_trm (x * 2)
+  | Fun_trm f ts => Fun_trm f (twilight_trms ts)
+  | Con_trm c =>
+    match c with
+    | inl cc => Con_trm c
+    | inr hc => Var_trm (hc * 2 + 1)
+    end
+  end.
+Proof.
+  destruct t; reflexivity.
+Defined.
+
+Lemma twilight_trms_unfold n (ts : trms L' n) :
+  twilight_trms ts =
+  match ts with
+  | O_trms => O_trms
+  | S_trms n t ts => S_trms n (twilight_trm t) (twilight_trms ts)
+  end.
+Proof.
+  destruct ts; reflexivity.
+Defined.
+
+#[local] Opaque Nat.mul Nat.div "mod".
+
+Lemma twilight_trm_fvs z (t : trm L')
+  : is_free_in_trm z t = is_free_in_trm (z * 2) (twilight_trm t)
+with twilight_trms_fvs n z (ts : trms L' n)
+  : is_free_in_trms z ts = is_free_in_trms (z * 2) (twilight_trms ts).
+Proof.
+  - trm_ind t; simpl.
+    + do 2 rewrite is_free_in_trm_unfold. obs_eqb x z; obs_eqb (x * 2) (z * 2); trivial; lia.
+    + do 2 rewrite is_free_in_trm_unfold. eapply twilight_trms_fvs.
+    + destruct c as [cc | hc]; do 2 rewrite is_free_in_trm_unfold; trivial.
+      obs_eqb (hc * 2 + 1) (z * 2); trivial. lia.
+  - trms_ind ts; simpl.
+    + do 2 rewrite is_free_in_trms_unfold. reflexivity.
+    + rewrite is_free_in_trms_unfold. rewrite twilight_trm_fvs. rewrite IH. reflexivity.
+Qed.
+
+Lemma twilight_trm_HC z (t : trm L')
+  : HC_occurs_in_trm z t = is_free_in_trm (z * 2 + 1) (twilight_trm t)
+with twilight_trms_HC n z (ts : trms L' n)
+  : HC_occurs_in_trms z ts = is_free_in_trms (z * 2 + 1) (twilight_trms ts).
+Proof.
+  - trm_ind t; simpl.
+    + rewrite is_free_in_trm_unfold. obs_eqb x z; obs_eqb (x * 2) (z * 2 + 1); trivial; lia.
+    + rewrite is_free_in_trm_unfold. rewrite HC_occurs_in_trm_Fun_trm. eapply twilight_trms_HC.
+    + destruct c as [cc | hc]; rewrite is_free_in_trm_unfold; rewrite HC_occurs_in_trm_Con_trm; trivial. obs_eqb z hc; obs_eqb (hc * 2 + 1) (z * 2 + 1); trivial; lia.
+  - trms_ind ts; simpl.
+    + rewrite is_free_in_trms_unfold. reflexivity.
+    + rewrite is_free_in_trms_unfold. rewrite HC_occurs_in_trms_S_trms. rewrite twilight_trm_HC. rewrite IH. reflexivity.
+Qed.
+
+Lemma twilight_trm_lemma sigma (t : trm L')
+  : hsubst_trm sigma t = subst_trm (twilight sigma) (twilight_trm t)
+with twilight_trms_lemma n sigma (ts : trms L' n)
+  : hsubst_trms sigma ts = subst_trms (twilight sigma) (twilight_trms ts).
+Proof.
+  - trm_ind t; simpl.
+    + rewrite subst_trm_unfold. unfold twilight. unfold enum. simpl.
+      exploit (@div_mod_uniqueness (x * 2) 2 x 0). rewrite Nat.mul_comm. lia. lia.
+      intros [-> ->]. simpl. reflexivity.
+    + rewrite subst_trm_unfold. f_equal. eapply twilight_trms_lemma.
+    + destruct c as [cc | hc].
+      * rewrite subst_trm_unfold. reflexivity.
+      * rewrite subst_trm_unfold. unfold twilight. unfold enum. simpl.
+        exploit (@div_mod_uniqueness (hc * 2 + 1) 2 hc 1). rewrite Nat.mul_comm. lia. lia.
+        intros [-> ->]. simpl. reflexivity.
+  - trms_ind ts; simpl.
+    + rewrite subst_trms_unfold. reflexivity.
+    + rewrite subst_trms_unfold. f_equal.
+      * eapply twilight_trm_lemma.
+      * eapply IH.
+Qed.
+
+Fixpoint twilight_frm (p : frm L') : frm L' :=
+  match p with
+  | Rel_frm R ts => Rel_frm R (twilight_trms ts)
+  | Eqn_frm t1 t2 => Eqn_frm (twilight_trm t1) (twilight_trm t2)
+  | Neg_frm p1 => Neg_frm (twilight_frm p1)
+  | Imp_frm p1 p2 => Imp_frm (twilight_frm p1) (twilight_frm p2)
+  | All_frm y p1 => All_frm (2 * y) (twilight_frm p1)
+  end.
+
+Lemma twilight_frm_fvs z (p : frm L')
+  : is_free_in_frm z p = is_free_in_frm (z * 2) (twilight_frm p).
+Proof.
+  frm_ind p; simpl.
+  - eapply twilight_trms_fvs.
+  - f_equal; eapply twilight_trm_fvs.
+  - eapply IH1.
+  - f_equal; [eapply IH1 | eapply IH2].
+  - f_equal; [eapply IH1 | f_equal]. rewrite Nat.mul_comm. obs_eqb z y; obs_eqb (2 * z) (2 * y); trivial; lia.
+Qed.
+
+Lemma twilight_frm_HC z (p : frm L')
+  : HC_occurs_in_frm z p = is_free_in_frm (z * 2 + 1) (twilight_frm p).
+Proof.
+  frm_ind p; simpl.
+  - eapply twilight_trms_HC.
+  - f_equal; eapply twilight_trm_HC.
+  - eapply IH1.
+  - f_equal; [eapply IH1 | eapply IH2].
+  - rewrite IH1. clear IH1. replace (negb (z * 2 + 1 =? 2 * y)) with true.
+    + destruct (is_free_in_frm (z * 2 + 1) (twilight_frm p1)) as [ | ]; trivial.
+    + symmetry. s!. lia.
+Qed.
+
+Lemma twilight_chi_frm sigma (p : frm L')
+  : hchi_frm sigma p = chi_frm (twilight sigma) (twilight_frm p).
+Proof.
+  unfold hchi_frm, chi_frm, twilight. f_equal. eapply maxs_ext. intros n. split.
+  - s!. intros [[x | hc] [EQ IN]].
+    + exists (x * 2). exploit (@div_mod_uniqueness (x * 2) 2 x 0). rewrite Nat.mul_comm. lia. lia.
+      intros [-> ->]. simpl. unfold id. rewrite EQ. split; trivial. s!. rewrite <- twilight_frm_fvs. now rewrite in_accum_hatom_in_frm_iff_is_free_in_frm in IN.
+    + exists (hc * 2 + 1). exploit (@div_mod_uniqueness (hc * 2 + 1) 2 hc 1). rewrite Nat.mul_comm. lia. lia.
+      intros [-> ->]. simpl. unfold id. rewrite EQ. split; trivial. s!. rewrite <- twilight_frm_HC. now rewrite in_accum_hatom_in_frm_iff_HC_occurs_in_frm in IN.
+  - s!. intros [x [EQ IN]]. exists (if x mod 2 =? 0 then inl (id (x / 2)) else inr (id (x / 2))). split; trivial. obs_eqb (x mod 2) 0.
+    + rewrite in_accum_hatom_in_frm_iff_is_free_in_frm. s!. rewrite twilight_frm_fvs. unfold id. replace (x / 2 * 2) with x; trivial. exploit (@Nat.div_mod x 2); lia.
+    + rewrite in_accum_hatom_in_frm_iff_HC_occurs_in_frm. s!. rewrite twilight_frm_HC. unfold id. replace (x / 2 * 2 + 1) with x; trivial. exploit (@Nat.div_mod x 2). lia. enough (WTS : x mod 2 = 1) by lia. exploit (Nat.mod_bound_pos x 2); lia.
+Qed.
+
+Lemma twilight_frm_lemma sigma (p : frm L')
+  : hsubst_frm sigma p = subst_frm (twilight sigma) (twilight_frm p).
+Proof.
+  revert sigma. frm_ind p; simpl; i.
+  - f_equal; eapply twilight_trms_lemma.
+  - f_equal; eapply twilight_trm_lemma.
+  - f_equal; eapply IH1.
+  - f_equal; [eapply IH1 | eapply IH2].
+  - rewrite IH1. rewrite twilight_chi_frm. f_equal. eapply equiv_subst_in_frm_implies_subst_frm_same.
+    intros u u_free. unfold twilight, cons_hsubst, cons_subst. simpl. obs_eqb (u mod 2) 0.
+    + destruct (eqb _ _) as [ | ] eqn: H_OBS'; rewrite eqb_spec in H_OBS'.
+      * destruct (eq_dec _ _) as [EQ | NE]; trivial. contradiction NE. hinv H_OBS'. unfold id. transitivity (2 * (u / 2) + u mod 2). eapply Nat.div_mod. lia. lia.
+      * destruct (eq_dec _ _) as [EQ | NE]; trivial. contradiction H_OBS'. f_equal. unfold id. rewrite EQ. symmetry. eapply Nat.div_unique with (r := 0). lia. lia.
+    + destruct (eqb _ _) as [ | ] eqn: H_OBS'; rewrite eqb_spec in H_OBS'.
+      * destruct (eq_dec _ _) as [EQ | NE]; trivial. congruence.
+      * destruct (eq_dec _ _) as [EQ | NE]; trivial. contradiction H_OBS. rewrite EQ. symmetry. eapply Nat.mod_unique with (q := y). lia. lia.
+Qed.
+
+End TWILIGHT.
 
 Context {enum_function_symbols : isEnumerable L.(function_symbols)} {enum_constant_symbols : isEnumerable L.(constant_symbols)} {enum_relation_symbols : isEnumerable L.(relation_symbols)}.
 
