theories/Logic/HilbertFol2.v
@@ -15,4 +15,26 @@ Module FolHilbert.
 
 Infix "⊢" := proves : type_scope.
 
+Section HENKIN.
+
+Context {L : language}.
+
+#[local] Notation L' := (augmented_language L Henkin_constants).
+
+#[local] Notation hatom := (ivar + Henkin_constants)%type.
+
+#[local] Notation hsubst := (hatom -> trm L').
+
+#[local] Existing Instance constant_symbols_similarity_instance.
+
+#[local] Existing Instance trm_similarity_instance.
+
+#[local] Existing Instance trms_similarity_instance.
+
+#[local] Existing Instance frm_similarity_instance.
+
+#[local] Existing Instance subst_similarity_instance.
+
+End HENKIN.
+
 End FolHilbert.
